@prefix : <https://github.com/andreazammarchi3/BeachVolleyballOntology/> .
@prefix owl: <http://www.w3.org/2002/07/owl#> .
@prefix rdf: <http://www.w3.org/1999/02/22-rdf-syntax-ns#> .
@prefix xml: <http://www.w3.org/XML/1998/namespace> .
@prefix xsd: <http://www.w3.org/2001/XMLSchema#> .
@prefix rdfs: <http://www.w3.org/2000/01/rdf-schema#> .
@prefix sport: <https://sportschema.org/ontologies/main/> .
@prefix schema: <https://schema.org/> .
@prefix spstat: <https://sportschema.org/ontologies/corestatistics/> .
@prefix dcterms: <http://purl.org/dc/terms/> .
@base <https://github.com/andreazammarchi3/BeachVolleyballOntology/> .

<https://github.com/andreazammarchi3/BeachVolleyballOntology/> rdf:type owl:Ontology ;
                                                                dcterms:creator "Andrea Zammarchi" ;
                                                                dcterms:description "An ontology for beach volleyball statistics and sports information." ;
                                                                dcterms:license "https://opensource.org/licenses/MIT" ;
                                                                dcterms:title "Beach Volleyball Ontology" ;
                                                                owl:versionInfo "1.0.0" .

#################################################################
#    Annotation properties
#################################################################

###  http://purl.org/dc/terms/creator
dcterms:creator rdf:type owl:AnnotationProperty .


###  http://purl.org/dc/terms/description
dcterms:description rdf:type owl:AnnotationProperty .


###  http://purl.org/dc/terms/license
dcterms:license rdf:type owl:AnnotationProperty .


###  http://purl.org/dc/terms/title
dcterms:title rdf:type owl:AnnotationProperty .


#################################################################
#    Datatypes
#################################################################

###  http://www.w3.org/2001/XMLSchema#date
xsd:date rdf:type rdfs:Datatype .


###  http://www.w3.org/2004/02/skos/core#Concept
<http://www.w3.org/2004/02/skos/core#Concept> rdf:type rdfs:Datatype .


#################################################################
#    Object Properties
#################################################################

###  https://sportschema.org/ontologies/corestatistics/resultEffectTarget
spstat:resultEffectTarget rdf:type owl:ObjectProperty ;
                          rdfs:domain sport:Participation ;
                          rdfs:range sport:ParticipatableThing .


###  https://sportschema.org/ontologies/main/actionInEvent
sport:actionInEvent rdf:type owl:ObjectProperty ;
                    owl:inverseOf sport:containsAction ;
                    rdfs:domain sport:Action ;
                    rdfs:range sport:Event ;
                    rdfs:comment "Link to the event in which an Action took place"@en ;
                    rdfs:isDefinedBy sport: ;
                    rdfs:label "action in event"@en .


###  https://sportschema.org/ontologies/main/child
sport:child rdf:type owl:ObjectProperty ;
            owl:inverseOf sport:parent ;
            rdfs:domain sport:ParticipatableThing ;
            rdfs:range sport:ParticipatableThing ;
            rdfs:comment "Link from a ParticipatableThing to its child, to represent child Event, CompetitionPhase etc"@en ;
            rdfs:isDefinedBy sport: ;
            rdfs:label "child"@en .


###  https://sportschema.org/ontologies/main/childSite
sport:childSite rdf:type owl:ObjectProperty ;
                owl:inverseOf sport:parentSite ;
                rdfs:domain sport:Site ;
                rdfs:range sport:Site ;
                rdfs:comment "Link from a Site to its child, such as a link from an Olympic Park to an individual stadium or from a tennis complex to an individual tennis court"@en ;
                rdfs:isDefinedBy sport: ;
                rdfs:label "child site"@en .


###  https://sportschema.org/ontologies/main/containsAction
sport:containsAction rdf:type owl:ObjectProperty ;
                     rdfs:domain sport:Event ;
                     rdfs:range sport:Action ;
                     rdfs:comment "Link to action in that took place at the Event"@en ;
                     rdfs:isDefinedBy sport: ;
                     rdfs:label "contains action"@en .


###  https://sportschema.org/ontologies/main/containsCompetitionPhase
sport:containsCompetitionPhase rdf:type owl:ObjectProperty ;
                               owl:inverseOf sport:phaseInCompetition ;
                               rdfs:domain sport:Competition ;
                               rdfs:range sport:CompetitionPhase ;
                               rdfs:comment "Link from the competition to its constituent phases"@en ;
                               rdfs:isDefinedBy sport: ;
                               rdfs:label "contains competition phase"@en .


###  https://sportschema.org/ontologies/main/containsEvent
sport:containsEvent rdf:type owl:ObjectProperty ;
                    owl:inverseOf sport:eventInCompetition ;
                    rdfs:domain sport:Competition ;
                    rdfs:range sport:Event ;
                    rdfs:comment "An Event that is part of this Competition"@en ;
                    rdfs:isDefinedBy sport: ;
                    rdfs:label "contains event"@en .


###  https://sportschema.org/ontologies/main/eventInCompetition
sport:eventInCompetition rdf:type owl:ObjectProperty ;
                         owl:inverseOf sport:phaseContainsEvent ;
                         rdfs:domain sport:Event ;
                         rdfs:range sport:Competition ;
                         rdfs:comment "The Competition that an Event is part of"@en ;
                         rdfs:isDefinedBy sport: ;
                         rdfs:label "event in competition"@en .


###  https://sportschema.org/ontologies/main/eventInCompetitionPhase
sport:eventInCompetitionPhase rdf:type owl:ObjectProperty ;
                              owl:inverseOf sport:phaseContainsEvent ;
                              rdfs:domain sport:Event ;
                              rdfs:range sport:CompetitionPhase ;
                              rdfs:comment "The CompetitionPhase (such as a round or a finals phase) of which an Event is a part"@en ;
                              rdfs:isDefinedBy sport: ;
                              rdfs:label "event in competition phase"@en .


###  https://sportschema.org/ontologies/main/governedBy
sport:governedBy rdf:type owl:ObjectProperty ;
                 owl:inverseOf sport:governs ;
                 rdfs:domain sport:Competition ;
                 rdfs:range sport:GoverningBody ;
                 rdfs:comment "Link to the organisation that regulates a given Competition"@en ;
                 rdfs:isDefinedBy sport: ;
                 rdfs:label "governing body"@en .


###  https://sportschema.org/ontologies/main/governs
sport:governs rdf:type owl:ObjectProperty ;
              rdfs:domain sport:GoverningBody ;
              rdfs:range sport:Competition ;
              rdfs:comment "Link to the competitions that the body governs."@en ;
              rdfs:isDefinedBy sport: ;
              rdfs:label "governs"@en .


###  https://sportschema.org/ontologies/main/location
sport:location rdf:type owl:ObjectProperty ;
               owl:inverseOf sport:locationOf ;
               rdfs:domain sport:ParticipatableThing ;
               rdfs:range sport:Site ;
               rdfs:comment "Link to the location (Site) where an event takes place"@en ;
               rdfs:isDefinedBy sport: ;
               rdfs:label "location"@en .


###  https://sportschema.org/ontologies/main/locationOf
sport:locationOf rdf:type owl:ObjectProperty ;
                 rdfs:domain sport:Site ;
                 rdfs:range sport:Event ;
                 rdfs:comment "Link to an event that takes place at this location (Site)"@en ;
                 rdfs:isDefinedBy sport: ;
                 rdfs:label "location of"@en .


###  https://sportschema.org/ontologies/main/member
sport:member rdf:type owl:ObjectProperty ;
             owl:inverseOf sport:memberOf ;
             rdfs:domain sport:IndividualMembership ;
             rdfs:range sport:Individual ;
             rdfs:comment "Link between a membership and an individual"@en ;
             rdfs:isDefinedBy sport: ;
             rdfs:label "member"@en .


###  https://sportschema.org/ontologies/main/memberOf
sport:memberOf rdf:type owl:ObjectProperty ;
               rdfs:domain sport:Individual ;
               rdfs:range sport:IndividualMembership ;
               rdfs:comment "Link between an individual and a membership"@en ;
               rdfs:isDefinedBy sport: ;
               rdfs:label "member of"@en .


###  https://sportschema.org/ontologies/main/membership
sport:membership rdf:type owl:ObjectProperty ;
                 owl:inverseOf sport:membershipOf ;
                 rdfs:domain sport:Team ;
                 rdfs:range sport:IndividualMembership ;
                 rdfs:comment "Link between a team and a membership"@en ;
                 rdfs:isDefinedBy sport: ;
                 rdfs:label "membership"@en .


###  https://sportschema.org/ontologies/main/membershipOf
sport:membershipOf rdf:type owl:ObjectProperty ;
                   rdfs:domain sport:IndividualMembership ;
                   rdfs:range sport:Team ;
                   rdfs:comment "Link between a membership and a team"@en ;
                   rdfs:isDefinedBy sport: ;
                   rdfs:label "membership of"@en .


###  https://sportschema.org/ontologies/main/parent
sport:parent rdf:type owl:ObjectProperty ;
             rdfs:domain sport:ParticipatableThing ;
             rdfs:range sport:ParticipatableThing ;
             rdfs:comment "Link from a ParticipatableThing to its parent, to represent parent Event, CompetitionPhase etc"@en ;
             rdfs:isDefinedBy sport: ;
             rdfs:label "parent"@en .


###  https://sportschema.org/ontologies/main/parentSite
sport:parentSite rdf:type owl:ObjectProperty ;
                 rdfs:domain sport:Site ;
                 rdfs:range sport:Site ;
                 rdfs:comment "Link from a Site to its parent, such as a link from a stadium to an Olympic Park or from a tennis court to the tennis complex"@en ;
                 rdfs:isDefinedBy sport: ;
                 rdfs:label "parent site"@en .


###  https://sportschema.org/ontologies/main/participantOf
sport:participantOf rdf:type owl:ObjectProperty ;
                    owl:inverseOf sport:participation ,
                                  sport:participationBy ;
                    rdfs:domain sport:Agent ;
                    rdfs:range sport:Participation ;
                    rdfs:comment "Link from a person or team to their participation in an event"@en ;
                    rdfs:isDefinedBy sport: ;
                    rdfs:label "participant of"@en .


###  https://sportschema.org/ontologies/main/participation
sport:participation rdf:type owl:ObjectProperty ;
                    owl:inverseOf sport:participationIn ;
                    rdfs:domain sport:ParticipatableThing ;
                    rdfs:range sport:Participation ;
                    rdfs:comment "Link from a ParticipatableThing to a participation by an Agent"@en ;
                    rdfs:isDefinedBy sport: ;
                    rdfs:label "participation"@en .


###  https://sportschema.org/ontologies/main/participationBy
sport:participationBy rdf:type owl:ObjectProperty ;
                      rdfs:domain sport:Participation ;
                      rdfs:range sport:Agent ;
                      rdfs:comment "Link to a person or team participating in an event, season or action"@en ;
                      rdfs:isDefinedBy sport: ;
                      rdfs:label "participation by"@en .


###  https://sportschema.org/ontologies/main/participationIn
sport:participationIn rdf:type owl:ObjectProperty ;
                      rdfs:domain sport:Participation ;
                      rdfs:range sport:ParticipatableThing ;
                      rdfs:comment "Link from a participation by an Agent to a ParticipatableThing"@en ;
                      rdfs:isDefinedBy sport: ;
                      rdfs:label "participation in"@en .


###  https://sportschema.org/ontologies/main/participationSplit
sport:participationSplit rdf:type owl:ObjectProperty ;
                         owl:inverseOf sport:participationSplitOf ;
                         rdfs:domain sport:Participation ;
                         rdfs:range sport:ParticipationSplit ;
                         rdfs:comment "Link to a part of a participation of an actor in an event or season, such as one half of a football match or all home games."@en ;
                         rdfs:isDefinedBy sport: ;
                         rdfs:label "participation split"@en .


###  https://sportschema.org/ontologies/main/participationSplitOf
sport:participationSplitOf rdf:type owl:ObjectProperty ;
                           rdfs:domain sport:ParticipationSplit ;
                           rdfs:range sport:Participation ;
                           rdfs:comment "Link to a participation of which this is a part"@en ;
                           rdfs:isDefinedBy sport: ;
                           rdfs:label "participation split of"@en .


###  https://sportschema.org/ontologies/main/phaseContainsEvent
sport:phaseContainsEvent rdf:type owl:ObjectProperty ;
                         rdfs:domain sport:CompetitionPhase ;
                         rdfs:range sport:Event ,
                                    sport:event ;
                         rdfs:comment "An Event (such as a round or a finals phase) contained in this CompetitionPhase"@en ,
                                      "The Event is part of a CompetitionPhase"@en ;
                         rdfs:isDefinedBy sport: ;
                         rdfs:label "phase contains event"@en .


###  https://sportschema.org/ontologies/main/phaseInCompetition
sport:phaseInCompetition rdf:type owl:ObjectProperty ;
                         rdfs:domain sport:CompetitionPhase ;
                         rdfs:range sport:Competition ;
                         rdfs:comment "Link to the competition of which this CompetitionPhase is a part"@en ;
                         rdfs:isDefinedBy sport: ;
                         rdfs:label "phase in competition"@en .


#################################################################
#    Data properties
#################################################################

###  https://sportschema.org/ontologies/corestatistics/adjustedScoreAgainst
spstat:adjustedScoreAgainst rdf:type owl:DatatypeProperty ;
                            rdfs:domain sport:Participation ;
                            rdfs:range xsd:integer ;
                            rdfs:comment "The final score against as adjusted by some authority. Usually as a result of some dispute or transgression that must be settled post-event and rendered in the score. Will differ from the regular score reflecting the number of actual goals scored in play. Should be tested for before displaying actual score."@en ;
                            rdfs:label "adjustedScoreAgainst"@en .


###  https://sportschema.org/ontologies/corestatistics/adjustedScoreFor
spstat:adjustedScoreFor rdf:type owl:DatatypeProperty ;
                        rdfs:domain sport:Participation ;
                        rdfs:range xsd:integer ;
                        rdfs:comment "The final score as adjusted by some authority. Usually as a result of some dispute or transgression that must be settled post-event and rendered in the score.  Will differ from the regular score reflecting the number of actual goals scored in play. Should be tested for before displaying actual score."@en ;
                        rdfs:label "adjustedScoreFor"@en .


###  https://sportschema.org/ontologies/corestatistics/eventOutcome
spstat:eventOutcome rdf:type owl:DatatypeProperty ;
                    rdfs:domain sport:Participation ;
                    rdfs:range xsd:integer ;
                    rdfs:comment "Whether the competitor won, lost, or tied."@en ;
                    rdfs:label "eventOutcome"@en .


###  https://sportschema.org/ontologies/corestatistics/eventStandingPoints
spstat:eventStandingPoints rdf:type owl:DatatypeProperty ;
                           rdfs:domain sport:Participation ;
                           rdfs:range xsd:integer ;
                           rdfs:comment "How many points were earned as a result of the outcome of this particular event."@en ;
                           rdfs:label "eventStandingPoints"@en .


###  https://sportschema.org/ontologies/corestatistics/eventStandingPointsAgainst
spstat:eventStandingPointsAgainst rdf:type owl:DatatypeProperty ;
                                  rdfs:domain sport:Participation ;
                                  rdfs:range xsd:integer ;
                                  rdfs:comment "How many points were deducted as a result of the outcome of this particular event. This occurs, for example, in the German Handball leagues."@en ;
                                  rdfs:label "eventStandingPointsAgainst"@en .


###  https://sportschema.org/ontologies/corestatistics/eventsDiscarded
spstat:eventsDiscarded rdf:type owl:DatatypeProperty ;
                       rdfs:domain sport:Participation ;
                       rdfs:range xsd:integer ;
                       rdfs:comment "The number of events that the team or player has discarded under this particular time period. Added from issue #29 2019-03-20."@en ;
                       rdfs:label "eventsDiscarded"@en .


###  https://sportschema.org/ontologies/corestatistics/eventsPlayed
spstat:eventsPlayed rdf:type owl:DatatypeProperty ;
                    rdfs:domain sport:Participation ;
                    rdfs:range xsd:integer ;
                    rdfs:comment "The number of sports-events in which this team or player has already participated."@en ;
                    rdfs:label "eventsPlayed"@en .


###  https://sportschema.org/ontologies/corestatistics/eventsRemaining
spstat:eventsRemaining rdf:type owl:DatatypeProperty ;
                       rdfs:domain sport:Participation ;
                       rdfs:range xsd:integer ;
                       rdfs:comment "Number of sports-events the player has yet to participate in."@en ;
                       rdfs:label "eventsRemaining"@en .


###  https://sportschema.org/ontologies/corestatistics/eventsStarted
spstat:eventsStarted rdf:type owl:DatatypeProperty ;
                     rdfs:domain sport:Participation ;
                     rdfs:range xsd:integer ;
                     rdfs:comment "Number of sports-events the player has played in since the start of the event."@en ;
                     rdfs:label "eventsStarted"@en .


###  https://sportschema.org/ontologies/corestatistics/gamesBack
spstat:gamesBack rdf:type owl:DatatypeProperty ;
                 rdfs:domain sport:Participation ;
                 rdfs:range xsd:integer ;
                 rdfs:comment "A number used to measure how behind one team is from first place. The first place team is 0 games back."@en ;
                 rdfs:label "gamesBack"@en .


###  https://sportschema.org/ontologies/corestatistics/losses
spstat:losses rdf:type owl:DatatypeProperty ;
              rdfs:domain sport:Participation ;
              rdfs:range xsd:integer ;
              rdfs:comment "Number of losses."@en ;
              rdfs:label "losses"@en .


###  https://sportschema.org/ontologies/corestatistics/lossesOvertime
spstat:lossesOvertime rdf:type owl:DatatypeProperty ;
                      rdfs:domain sport:Participation ;
                      rdfs:range xsd:integer ;
                      rdfs:comment "Number of losses in events which went into overtime. For leagues that use this as a top-level outcome category (eg. NHL), as opposed to just a derivative of scoping."@en ;
                      rdfs:label "lossesOvertime"@en .


###  https://sportschema.org/ontologies/corestatistics/periodExtraTimeAdded
spstat:periodExtraTimeAdded rdf:type owl:DatatypeProperty ;
                            rdfs:domain sport:Participation ;
                            rdfs:range xsd:integer ;
                            rdfs:comment "How many minutes the referee has decided to add to the period."@en ;
                            rdfs:label "periodExtraTimeAdded"@en .


###  https://sportschema.org/ontologies/corestatistics/periodExtraTimeElapsed
spstat:periodExtraTimeElapsed rdf:type owl:DatatypeProperty ;
                              rdfs:domain sport:Participation ;
                              rdfs:range xsd:integer ;
                              rdfs:comment "How much time exactly MMSS that was actually elapsed in the period."@en ;
                              rdfs:label "periodExtraTimeElapsed"@en .


###  https://sportschema.org/ontologies/corestatistics/points
spstat:points rdf:type owl:DatatypeProperty ;
              rdfs:domain sport:Participation ;
              rdfs:range xsd:integer ;
              rdfs:comment "Points accumulated by this associate. For example, points earned by a NASCAR owner."@en ;
              rdfs:label "points"@en .


###  https://sportschema.org/ontologies/corestatistics/pointsDifference
spstat:pointsDifference rdf:type owl:DatatypeProperty ;
                        rdfs:domain sport:Participation ;
                        rdfs:range xsd:integer ;
                        rdfs:comment "The final calculated difference between points-scored-for and points-scored-against. Possibly takes into account other scoring aspects, such as penalties and differences in score-values."@en ;
                        rdfs:label "pointsDifference"@en .


###  https://sportschema.org/ontologies/corestatistics/pointsScoredAgainst
spstat:pointsScoredAgainst rdf:type owl:DatatypeProperty ;
                           rdfs:domain sport:Participation ;
                           rdfs:range xsd:integer ;
                           rdfs:comment "The number of points scored against a team by its opponents during an extended time period."@en ;
                           rdfs:label "pointsScoredAgainst"@en .


###  https://sportschema.org/ontologies/corestatistics/pointsScoredFor
spstat:pointsScoredFor rdf:type owl:DatatypeProperty ;
                       rdfs:domain sport:Participation ;
                       rdfs:range xsd:integer ;
                       rdfs:comment "The number of points a team has scored against its opponents during an extended time period."@en ;
                       rdfs:label "pointsScoredFor"@en .


###  https://sportschema.org/ontologies/corestatistics/rating
spstat:rating rdf:type owl:DatatypeProperty ;
              rdfs:domain sport:Participation ;
              rdfs:range xsd:string ;
              rdfs:comment "A judged value placed on the team or individual. Often used in British soccer."@en ;
              rdfs:label "rating"@en .


###  https://sportschema.org/ontologies/corestatistics/relegationAverage
spstat:relegationAverage rdf:type owl:DatatypeProperty ;
                         rdfs:domain sport:Participation ;
                         rdfs:range xsd:integer ;
                         rdfs:comment "The product of a relegation average formula used to determine which team is demoted to a lower league. The formula may vary by league but the average typically looks at team performance across multiple competitions. The team(s) with the lowest relegation averages is sent to the league below."@en ;
                         rdfs:label "relegationAverage"@en .


###  https://sportschema.org/ontologies/corestatistics/resultEffect
spstat:resultEffect rdf:type owl:DatatypeProperty ;
                    rdfs:domain sport:Participation ;
                    rdfs:range xsd:anyURI ;
                    rdfs:comment "Describes the effect that the result of the event or rank changing has had on the team. Example: Whether or not a team has qualified for the playoffs, or has been promoted or demoted to a different division. Value should come from the https://cv.iptc.org/newscodes/spresulteffect/ vocabulary"@en ;
                    rdfs:label "resultEffect"@en .


###  https://sportschema.org/ontologies/corestatistics/resultEffectTarget
spstat:resultEffectTarget rdf:type owl:DatatypeProperty .


###  https://sportschema.org/ontologies/corestatistics/score
spstat:score rdf:type owl:DatatypeProperty ;
             rdfs:domain sport:Participation ;
             rdfs:range xsd:integer ;
             rdfs:comment "Final or current score of the team or player."@en ;
             rdfs:label "score"@en .


###  https://sportschema.org/ontologies/corestatistics/scoreAttempts
spstat:scoreAttempts rdf:type owl:DatatypeProperty ;
                     rdfs:domain sport:Participation ;
                     rdfs:range xsd:integer ;
                     rdfs:comment "Final or current number of attempts to score by a team or player. Example: in ice hockey, would represent total shots on goal."@en ;
                     rdfs:label "scoreAttempts"@en .


###  https://sportschema.org/ontologies/corestatistics/scoreAttemptsOnGoal
spstat:scoreAttemptsOnGoal rdf:type owl:DatatypeProperty ;
                           rdfs:domain sport:Participation ;
                           rdfs:range xsd:integer ;
                           rdfs:comment "A subset of score-attempts. Only counts those attempts that were on-goal."@en ;
                           rdfs:label "scoreAttemptsOnGoal"@en .


###  https://sportschema.org/ontologies/corestatistics/scoreAttemptsOnGoalOpposing
spstat:scoreAttemptsOnGoalOpposing rdf:type owl:DatatypeProperty ;
                                   rdfs:domain sport:Participation ;
                                   rdfs:range xsd:integer ;
                                   rdfs:comment "Final or current number of attempts to score by an opposing team or player that were on-goal."@en ;
                                   rdfs:label "scoreAttemptsOnGoalOpposing"@en .


###  https://sportschema.org/ontologies/corestatistics/scoreAttemptsOpposing
spstat:scoreAttemptsOpposing rdf:type owl:DatatypeProperty ;
                             rdfs:domain sport:Participation ;
                             rdfs:range xsd:integer ;
                             rdfs:comment "Final or current number of attempts to score by an opposing team or player."@en ;
                             rdfs:label "scoreAttemptsOpposing"@en .


###  https://sportschema.org/ontologies/corestatistics/scoreAverage
spstat:scoreAverage rdf:type owl:DatatypeProperty ;
                    rdfs:domain sport:Participation ;
                    rdfs:range xsd:integer ;
                    rdfs:comment "Average per-game score for the team or player."@en ;
                    rdfs:label "scoreAverage"@en .


###  https://sportschema.org/ontologies/corestatistics/scoreBehind
spstat:scoreBehind rdf:type owl:DatatypeProperty ;
                   rdfs:domain sport:Participation ;
                   rdfs:range xsd:integer ;
                   rdfs:comment "The points or time behind the leading score."@en ;
                   rdfs:label "scoreBehind"@en .


###  https://sportschema.org/ontologies/corestatistics/scoreOpposing
spstat:scoreOpposing rdf:type owl:DatatypeProperty ;
                     rdfs:domain sport:Participation ;
                     rdfs:range xsd:integer ;
                     rdfs:comment "Final or current score of the opposing team or player."@en ;
                     rdfs:label "scoreOpposing"@en .


###  https://sportschema.org/ontologies/corestatistics/scoreOpposingAverage
spstat:scoreOpposingAverage rdf:type owl:DatatypeProperty ;
                            rdfs:domain sport:Participation ;
                            rdfs:range xsd:integer ;
                            rdfs:comment "Average per-game score for the opposing team or player."@en ;
                            rdfs:label "scoreOpposingAverage"@en .


###  https://sportschema.org/ontologies/corestatistics/scorePercentage
spstat:scorePercentage rdf:type owl:DatatypeProperty ;
                       rdfs:domain sport:Participation ;
                       rdfs:range xsd:integer ;
                       rdfs:comment "Percentage of attempted scores that reached their mark."@en ;
                       rdfs:label "scorePercentage"@en .


###  https://sportschema.org/ontologies/corestatistics/scorePercentageOpposing
spstat:scorePercentageOpposing rdf:type owl:DatatypeProperty ;
                               rdfs:domain sport:Participation ;
                               rdfs:range xsd:integer ;
                               rdfs:comment "Percentage of attempted scores by opposing team or player that reached their mark."@en ;
                               rdfs:label "scorePercentageOpposing"@en .


###  https://sportschema.org/ontologies/corestatistics/seriesScore
spstat:seriesScore rdf:type owl:DatatypeProperty ;
                   rdfs:domain sport:Participation ;
                   rdfs:range xsd:integer ;
                   rdfs:comment "Number of events in a series won by team or player."@en ;
                   rdfs:label "seriesScore"@en .


###  https://sportschema.org/ontologies/corestatistics/seriesScoreOpposing
spstat:seriesScoreOpposing rdf:type owl:DatatypeProperty ;
                           rdfs:domain sport:Participation ;
                           rdfs:range xsd:integer ;
                           rdfs:comment "Number of events in a series won by opposing team or player."@en ;
                           rdfs:label "seriesScoreOpposing"@en .


###  https://sportschema.org/ontologies/corestatistics/standingPoints
spstat:standingPoints rdf:type owl:DatatypeProperty ;
                      rdfs:domain sport:Participation ;
                      rdfs:range xsd:integer ;
                      rdfs:comment "A quantity used to rank teams, usually within a division, in order to decide who comes in first at the end of a season. Localized to the coverage-attributes."@en ;
                      rdfs:label "standingPoints"@en .


###  https://sportschema.org/ontologies/corestatistics/standingPointsAgainst
spstat:standingPointsAgainst rdf:type owl:DatatypeProperty ;
                             rdfs:domain sport:Participation ;
                             rdfs:range xsd:integer ;
                             rdfs:comment "Points counted against a team in rankings. Used in European handball standings, for example."@en ;
                             rdfs:label "standingPointsAgainst"@en .


###  https://sportschema.org/ontologies/corestatistics/streakDuration
spstat:streakDuration rdf:type owl:DatatypeProperty ;
                      rdfs:domain sport:Participation ;
                      rdfs:range xsd:integer ;
                      rdfs:comment "How long the streak lasted."@en ;
                      rdfs:label "streakDuration"@en .


###  https://sportschema.org/ontologies/corestatistics/streakEnd
spstat:streakEnd rdf:type owl:DatatypeProperty ;
                 rdfs:domain sport:Participation ;
                 rdfs:range xsd:integer ;
                 rdfs:comment "Date on which the streak ended."@en ;
                 rdfs:label "streakEnd"@en .


###  https://sportschema.org/ontologies/corestatistics/streakStart
spstat:streakStart rdf:type owl:DatatypeProperty ;
                   rdfs:domain sport:Participation ;
                   rdfs:range xsd:integer ;
                   rdfs:comment "Date on which the streak began."@en ;
                   rdfs:label "streakStart"@en .


###  https://sportschema.org/ontologies/corestatistics/streakTotal
spstat:streakTotal rdf:type owl:DatatypeProperty ;
                   rdfs:domain sport:Participation ;
                   rdfs:range xsd:integer ;
                   rdfs:comment "Holds the number of goals scored during a streak-type of score, for example."@en ;
                   rdfs:label "streakTotal"@en .


###  https://sportschema.org/ontologies/corestatistics/ties
spstat:ties rdf:type owl:DatatypeProperty ;
            rdfs:domain sport:Participation ;
            rdfs:range xsd:integer ;
            rdfs:comment "Number of ties."@en ;
            rdfs:label "ties"@en .


###  https://sportschema.org/ontologies/corestatistics/timeOfPossession
spstat:timeOfPossession rdf:type owl:DatatypeProperty ;
                        rdfs:domain sport:Participation ;
                        rdfs:range xsd:integer ;
                        rdfs:comment "Amount of time the team or player has possession of ball (or similar object like puck)."@en ;
                        rdfs:label "timeOfPossession"@en .


###  https://sportschema.org/ontologies/corestatistics/timeOfPossessionAverage
spstat:timeOfPossessionAverage rdf:type owl:DatatypeProperty ;
                               rdfs:domain sport:Participation ;
                               rdfs:range xsd:integer ;
                               rdfs:comment "Amount of time the team or player has possession of ball (or similar object like puck) per game."@en ;
                               rdfs:label "timeOfPossessionAverage"@en .


###  https://sportschema.org/ontologies/corestatistics/timeOfPossessionAverageOpposing
spstat:timeOfPossessionAverageOpposing rdf:type owl:DatatypeProperty ;
                                       rdfs:domain sport:Participation ;
                                       rdfs:range xsd:integer ;
                                       rdfs:comment "Amount of time the opposing team or player has possession of ball (or similar object like puck) per game."@en ;
                                       rdfs:label "timeOfPossessionAverageOpposing"@en .


###  https://sportschema.org/ontologies/corestatistics/timeOfPossessionPercentage
spstat:timeOfPossessionPercentage rdf:type owl:DatatypeProperty ;
                                  rdfs:domain sport:Participation ;
                                  rdfs:range xsd:integer ;
                                  rdfs:comment "Amount of time the team or player has possession of ball (or similar object like puck) expressed as a percentage of the full time of the match."@en ;
                                  rdfs:label "timeOfPossessionPercentage"@en .


###  https://sportschema.org/ontologies/corestatistics/timeOfPossessionPercentageOpposing
spstat:timeOfPossessionPercentageOpposing rdf:type owl:DatatypeProperty ;
                                          rdfs:domain sport:Participation ;
                                          rdfs:range xsd:integer ;
                                          rdfs:comment "Amount of time the opposing team or player has possession of ball (or similar object like puck) expressed as a percentage of the full time of the match."@en ;
                                          rdfs:label "timeOfPossessionPercentageOpposing"@en .


###  https://sportschema.org/ontologies/corestatistics/timePlayedEvent
spstat:timePlayedEvent rdf:type owl:DatatypeProperty ;
                       rdfs:domain sport:Participation ;
                       rdfs:range xsd:integer ;
                       rdfs:comment "Value for the amount of time played by this player in a particular sports-event."@en ;
                       rdfs:label "timePlayedEvent"@en .


###  https://sportschema.org/ontologies/corestatistics/timePlayedEventAverage
spstat:timePlayedEventAverage rdf:type owl:DatatypeProperty ;
                              rdfs:domain sport:Participation ;
                              rdfs:range xsd:integer ;
                              rdfs:comment "Value for the average amount of time played per-event by the player over the course of a particular time-span, such as a season."@en ;
                              rdfs:label "timePlayedEventAverage"@en .


###  https://sportschema.org/ontologies/corestatistics/timePlayedTotal
spstat:timePlayedTotal rdf:type owl:DatatypeProperty ;
                       rdfs:domain sport:Participation ;
                       rdfs:range xsd:integer ;
                       rdfs:comment "Value for the amount of time played by the team or player over the course of a particular time-span, such as a season."@en ;
                       rdfs:label "timePlayedTotal"@en .


###  https://sportschema.org/ontologies/corestatistics/undecideds
spstat:undecideds rdf:type owl:DatatypeProperty ;
                  rdfs:domain sport:Participation ;
                  rdfs:range xsd:integer ;
                  rdfs:comment "Number of events that were started, but ended up undecided."@en ;
                  rdfs:label "undecideds"@en .


###  https://sportschema.org/ontologies/corestatistics/winningPercentage
spstat:winningPercentage rdf:type owl:DatatypeProperty ;
                         rdfs:domain sport:Participation ;
                         rdfs:range xsd:integer ;
                         rdfs:comment "The winning percentage. Generally, wins divided by total events completed."@en ;
                         rdfs:label "winningPercentage"@en .


###  https://sportschema.org/ontologies/corestatistics/wins
spstat:wins rdf:type owl:DatatypeProperty ;
            rdfs:domain sport:Participation ;
            rdfs:range xsd:integer ;
            rdfs:comment "Number of wins."@en ;
            rdfs:label "wins"@en .


###  https://sportschema.org/ontologies/main/actionDateTime
sport:actionDateTime rdf:type owl:DatatypeProperty ;
                     rdfs:domain sport:Action ;
                     rdfs:range xsd:dateTime ;
                     rdfs:comment "Date and time when this play/action took place on the field."@en ;
                     rdfs:isDefinedBy sport: ;
                     rdfs:label "action date-time"@en .


###  https://sportschema.org/ontologies/main/actionType
sport:actionType rdf:type owl:DatatypeProperty ;
                 rdfs:domain sport:Action ;
                 rdfs:range <http://www.w3.org/2004/02/skos/core#Concept> ;
                 rdfs:comment "The type of competitive action taken on the field of play. See 'action' SportsML vocabs for various sports: http://cv.iptc.org/newscodes/spamfaction/ http://cv.iptc.org/newscodes/spbblaction/ http://cv.iptc.org/newscodes/spbkbaction/ http://cv.iptc.org/newscodes/spichaction/ http://cv.iptc.org/newscodes/spmcraction/ http://cv.iptc.org/newscodes/rgxaction/ http://cv.iptc.org/newscodes/spsocaction/ http://cv.iptc.org/newscodes/sptenaction/"@en ;
                 rdfs:isDefinedBy sport: ;
                 rdfs:label "action type"@en .


###  https://sportschema.org/ontologies/main/alignment
sport:alignment rdf:type owl:DatatypeProperty ;
                rdfs:domain sport:TeamParticipation ;
                rdfs:range xsd:anyURI ;
                rdfs:comment "The association between a Team and a Site, e.g. 'home' or 'away'"@en ;
                rdfs:isDefinedBy sport: ;
                rdfs:label "alignment"@en .


###  https://sportschema.org/ontologies/main/angle
sport:angle rdf:type owl:DatatypeProperty ;
            rdfs:domain sport:Action ;
            rdfs:range xsd:string ;
            rdfs:comment "Angle on the field of the play."@en ;
            rdfs:isDefinedBy sport: ;
            rdfs:label "angle"@en .


###  https://sportschema.org/ontologies/main/attendance
sport:attendance rdf:type owl:DatatypeProperty ;
                 rdfs:domain sport:Event ;
                 rdfs:range xsd:string ;
                 rdfs:comment "The number of people attending an event"@en ;
                 rdfs:isDefinedBy sport: ;
                 rdfs:label "attendance"@en .


###  https://sportschema.org/ontologies/main/bodyPart
sport:bodyPart rdf:type owl:DatatypeProperty ;
               rdfs:domain sport:Action ;
               rdfs:range xsd:string ;
               rdfs:comment "Body part used to perform an action."@en ;
               rdfs:isDefinedBy sport: ;
               rdfs:label "body part"@en .


###  https://sportschema.org/ontologies/main/class
sport:class rdf:type owl:DatatypeProperty ;
            rdfs:domain sport:Action ;
            rdfs:range <http://www.w3.org/2004/02/skos/core#Concept> ;
            rdfs:comment "An open placeholder for categorization. Recommended vocabulary: http://cv.iptc.org/newscodes/spactionclass/"@en ;
            rdfs:isDefinedBy sport: ;
            rdfs:label "class"@en .


###  https://sportschema.org/ontologies/main/comment
sport:comment rdf:type owl:DatatypeProperty ;
              rdfs:domain sport:Action ;
              rdfs:range xsd:string ;
              rdfs:comment "Textual comment of the action"@en ;
              rdfs:isDefinedBy sport: ;
              rdfs:label "comment"@en .


###  https://sportschema.org/ontologies/main/competitionFormat
sport:competitionFormat rdf:type owl:DatatypeProperty ;
                        rdfs:domain sport:CompetitionPhase ;
                        rdfs:range <http://www.w3.org/2004/02/skos/core#Concept> ;
                        rdfs:comment "Competition format: round robin, sudden death etc"@en ;
                        rdfs:isDefinedBy sport: ;
                        rdfs:label "competition form"@en .


###  https://sportschema.org/ontologies/main/competitionPhaseType
sport:competitionPhaseType rdf:type owl:DatatypeProperty ;
                           rdfs:domain sport:CompetitionPhase ;
                           rdfs:range <http://www.w3.org/2004/02/skos/core#Concept> ;
                           rdfs:comment "Type of the competition phase - regular week, final etc"@en ;
                           rdfs:isDefinedBy sport: ;
                           rdfs:label "competition phase type"@en .


###  https://sportschema.org/ontologies/main/competitionType
sport:competitionType rdf:type owl:DatatypeProperty ;
                      rdfs:domain sport:Competition ;
                      rdfs:range <http://www.w3.org/2004/02/skos/core#Concept> ;
                      rdfs:comment "The type of a Competition, e.g. spct:recurring-competition or spct:competition"@en ;
                      rdfs:isDefinedBy sport: ;
                      rdfs:label "competition type"@en .


###  https://sportschema.org/ontologies/main/dateOfBirth
sport:dateOfBirth rdf:type owl:DatatypeProperty ;
                  rdfs:domain sport:Individual ;
                  rdfs:range xsd:date ;
                  rdfs:comment "The date of birth of a person"@en ;
                  rdfs:isDefinedBy sport: ;
                  rdfs:label "date of birth"@en .


###  https://sportschema.org/ontologies/main/distance
sport:distance rdf:type owl:DatatypeProperty ;
               rdfs:domain sport:Action ;
               rdfs:range xsd:string ;
               rdfs:comment "Distance of the action."@en ;
               rdfs:isDefinedBy sport: ;
               rdfs:label "distance"@en .


###  https://sportschema.org/ontologies/main/endDate
sport:endDate rdf:type owl:DatatypeProperty ;
              rdfs:domain sport:Membership ;
              rdfs:range xsd:date ;
              rdfs:comment "The date on which a membership ends"@en ;
              rdfs:isDefinedBy sport: ;
              rdfs:label "end date"@en .


###  https://sportschema.org/ontologies/main/endDateTime
sport:endDateTime rdf:type owl:DatatypeProperty ;
                  rdfs:domain sport:Event ;
                  rdfs:range xsd:dateTime ;
                  rdfs:comment "The date and time at which an event ends"@en ;
                  rdfs:isDefinedBy sport: ;
                  rdfs:label "end datetime"@en .


###  https://sportschema.org/ontologies/main/endLocation
sport:endLocation rdf:type owl:DatatypeProperty ;
                  rdfs:domain sport:Action ;
                  rdfs:range xsd:string ;
                  rdfs:comment "A string indicating where on the court the action occured. Could be an approximate region, or a more complex value adhering to some elaborate coordinate system."@en ;
                  rdfs:isDefinedBy sport: ;
                  rdfs:label "end location"@en .


###  https://sportschema.org/ontologies/main/eventOutcome
sport:eventOutcome rdf:type owl:DatatypeProperty ;
                   rdfs:domain sport:CompetitorParticipation ;
                   rdfs:range <http://www.w3.org/2004/02/skos/core#Concept> ;
                   rdfs:comment "The outcome of an event (win, loss etc)"@en ;
                   rdfs:isDefinedBy sport: ;
                   rdfs:label "event outcome"@en .


###  https://sportschema.org/ontologies/main/eventOutcomeType
sport:eventOutcomeType rdf:type owl:DatatypeProperty ;
                       rdfs:domain sport:CompetitorParticipation ;
                       rdfs:range <http://www.w3.org/2004/02/skos/core#Concept> ;
                       rdfs:comment "The type of outcome of an event (win, loss etc)"@en ;
                       rdfs:isDefinedBy sport: ;
                       rdfs:label "event outcome type"@en .


###  https://sportschema.org/ontologies/main/eventStatus
sport:eventStatus rdf:type owl:DatatypeProperty ;
                  rdfs:domain sport:Event ;
                  rdfs:range <http://www.w3.org/2004/02/skos/core#Concept> ;
                  rdfs:comment "Event's current status (e.g. post-event)"@en ;
                  rdfs:isDefinedBy sport: ;
                  rdfs:label "event status"@en .


###  https://sportschema.org/ontologies/main/fieldLocation
sport:fieldLocation rdf:type owl:DatatypeProperty ;
                    rdfs:domain sport:Action ;
                    rdfs:range xsd:string ;
                    rdfs:comment "Recommended x,y 0-100. The location of the action on the field of play represented as a grid."@en ;
                    rdfs:isDefinedBy sport: ;
                    rdfs:label "field location"@en .


###  https://sportschema.org/ontologies/main/goalLocation
sport:goalLocation rdf:type owl:DatatypeProperty ;
                   rdfs:domain sport:Action ;
                   rdfs:range xsd:string ;
                   rdfs:comment "Recommended x,y 0-100. The location on goal-mouth grid in which the ball/puck entered."@en ;
                   rdfs:isDefinedBy sport: ;
                   rdfs:label "goal location"@en .


###  https://sportschema.org/ontologies/main/infractionLevel
sport:infractionLevel rdf:type owl:DatatypeProperty ;
                      rdfs:domain sport:Action ;
                      rdfs:range xsd:string ;
                      rdfs:comment "Level of infraction (aka penalty)"@en ;
                      rdfs:isDefinedBy sport: ;
                      rdfs:label "infraction level"@en .


###  https://sportschema.org/ontologies/main/infractionType
sport:infractionType rdf:type owl:DatatypeProperty ;
                     rdfs:domain sport:Action ;
                     rdfs:range <http://www.w3.org/2004/02/skos/core#Concept> ;
                     rdfs:comment "The degree of punishment for the infraction/penalty eg. yellow or red card, major, minor, game misconduct, etc. See 'penaltylevel' SportsML vocabs for various sports: http://cv.iptc.org/newscodes/spbkbpenaltylevel/ http://cv.iptc.org/newscodes/spichpenaltylevel/ http://cv.iptc.org/newscodes/sprgxpenaltylevel/ http://cv.iptc.org/newscodes/spsocpenaltylevel/"@en ;
                     rdfs:isDefinedBy sport: ;
                     rdfs:label "infraction type"@en .


###  https://sportschema.org/ontologies/main/lastModified
sport:lastModified rdf:type owl:DatatypeProperty ;
                   rdfs:domain sport:Action ;
                   rdfs:range xsd:string ;
                   rdfs:comment "Date and time when this play/action record was last modified. This would be the record from the reporter's data entry system."@en ;
                   rdfs:isDefinedBy sport: ;
                   rdfs:label "last modified"@en .


###  https://sportschema.org/ontologies/main/membershipStatus
sport:membershipStatus rdf:type owl:DatatypeProperty ;
                       rdfs:domain sport:IndividualMembership ;
                       rdfs:range <http://www.w3.org/2004/02/skos/core#Concept> ;
                       rdfs:comment "Member's status in a team during this membership period (e.g. active or inactive)"@en ;
                       rdfs:isDefinedBy sport: ;
                       rdfs:label "membership status"@en .


###  https://sportschema.org/ontologies/main/minutesElapsed
sport:minutesElapsed rdf:type owl:DatatypeProperty ;
                     rdfs:domain sport:Action ;
                     rdfs:range xsd:string ;
                     rdfs:comment "Game minutes elapsed when this action occurred"@en ;
                     rdfs:isDefinedBy sport: ;
                     rdfs:label "minutes elapsed"@en .


###  https://sportschema.org/ontologies/main/nationality
sport:nationality rdf:type owl:DatatypeProperty ;
                  rdfs:domain sport:Individual ;
                  rdfs:range xsd:string ;
                  rdfs:comment "The country an individual is identified with"@en ;
                  rdfs:isDefinedBy sport: ;
                  rdfs:label "nationality"@en .


###  https://sportschema.org/ontologies/main/participationSplitType
sport:participationSplitType rdf:type owl:DatatypeProperty ;
                             rdfs:domain sport:ParticipationSplit ;
                             rdfs:range xsd:anyURI ;
                             rdfs:comment "The type of a participation split, e.g. 'home games' or 'first half'"@en ;
                             rdfs:isDefinedBy sport: ;
                             rdfs:label "participation split type"@en .


###  https://sportschema.org/ontologies/main/passDescription
sport:passDescription rdf:type owl:DatatypeProperty ;
                      rdfs:domain sport:Action ;
                      rdfs:range xsd:string ;
                      rdfs:comment "description of the pass taken in this action"@en ;
                      rdfs:isDefinedBy sport: ;
                      rdfs:label "pass description"@en .


###  https://sportschema.org/ontologies/main/passMethod
sport:passMethod rdf:type owl:DatatypeProperty ;
                 rdfs:domain sport:Action ;
                 rdfs:range xsd:string ;
                 rdfs:comment "Method used in this pass"@en ;
                 rdfs:isDefinedBy sport: ;
                 rdfs:label "pass method"@en .


###  https://sportschema.org/ontologies/main/passType
sport:passType rdf:type owl:DatatypeProperty ;
               rdfs:domain sport:Action ;
               rdfs:range xsd:string ;
               rdfs:comment "Type of this pass"@en ;
               rdfs:isDefinedBy sport: ;
               rdfs:label "pass type"@en .


###  https://sportschema.org/ontologies/main/periodValue
sport:periodValue rdf:type owl:DatatypeProperty ;
                  rdfs:domain sport:Action ;
                  rdfs:range xsd:string ;
                  rdfs:comment "Used for tracking stats and events by period."@en ;
                  rdfs:isDefinedBy sport: ;
                  rdfs:label "period value"@en .


###  https://sportschema.org/ontologies/main/personReplacingPosition
sport:personReplacingPosition rdf:type owl:DatatypeProperty ;
                              rdfs:domain sport:Action ;
                              rdfs:range xsd:string ;
                              rdfs:comment "The position role assumed by the substitute."@en ;
                              rdfs:isDefinedBy sport: ;
                              rdfs:label "person replacing position"@en .


###  https://sportschema.org/ontologies/main/playerStatus
sport:playerStatus rdf:type owl:DatatypeProperty ;
                   rdfs:domain sport:IndividualParticipation ;
                   rdfs:range <http://www.w3.org/2004/02/skos/core#Concept> ;
                   rdfs:comment "Player status for a given event (e.g. starter or bench)"@en ;
                   rdfs:isDefinedBy sport: ;
                   rdfs:label "player status"@en .


###  https://sportschema.org/ontologies/main/positionEvent
sport:positionEvent rdf:type owl:DatatypeProperty ;
                    rdfs:domain sport:CompetitorParticipation ;
                    rdfs:range <http://www.w3.org/2004/02/skos/core#Concept> ;
                    rdfs:comment "The position in a team taken for an individual event"@en ;
                    rdfs:isDefinedBy sport: ;
                    rdfs:label "position (event)"@en .


###  https://sportschema.org/ontologies/main/positionRegular
sport:positionRegular rdf:type owl:DatatypeProperty ;
                      rdfs:domain sport:IndividualMembership ;
                      rdfs:range <http://www.w3.org/2004/02/skos/core#Concept> ;
                      rdfs:comment "The position in a team usually taken by a given player or associate"@en ;
                      rdfs:isDefinedBy sport: ;
                      rdfs:label "position (regular)"@en .


###  https://sportschema.org/ontologies/main/rank
sport:rank rdf:type owl:DatatypeProperty ;
           rdfs:domain sport:CompetitorParticipation ;
           rdfs:range xsd:string ;
           rdfs:comment "The rank of a player or team in standings etc."@en ;
           rdfs:isDefinedBy sport: ;
           rdfs:label "rank"@en .


###  https://sportschema.org/ontologies/main/recipientType
sport:recipientType rdf:type owl:DatatypeProperty ;
                    rdfs:domain sport:Action ;
                    rdfs:range <http://www.w3.org/2004/02/skos/core#Concept> ;
                    rdfs:comment "Whether the receiver of the penalty was the team, the player, a coach, a ref, etc. SportsML vocab uri: http://cv.iptc.org/newscodes/sprecipienttype/"@en ;
                    rdfs:isDefinedBy sport: ;
                    rdfs:label "recipient type"@en .


###  https://sportschema.org/ontologies/main/result
sport:result rdf:type owl:DatatypeProperty ;
             rdfs:domain sport:Action ;
             rdfs:range <http://www.w3.org/2004/02/skos/core#Concept> ;
             rdfs:comment "The result of the play or action. See 'result' SportsML vocabs for various sports: http://cv.iptc.org/newscodes/spamfresult/ http://cv.iptc.org/newscodes/spsocresult/"@en ;
             rdfs:isDefinedBy sport: ;
             rdfs:label "result"@en .


###  https://sportschema.org/ontologies/main/role
sport:role rdf:type owl:DatatypeProperty ;
           rdfs:domain sport:Participation ;
           rdfs:range <http://www.w3.org/2004/02/skos/core#Concept> ;
           rdfs:comment "A team's or individual's role in a given action"@en ;
           rdfs:isDefinedBy sport: ;
           rdfs:label "role"@en .


###  https://sportschema.org/ontologies/main/saveMethod
sport:saveMethod rdf:type owl:DatatypeProperty ;
                 rdfs:domain sport:Action ;
                 rdfs:range xsd:string ;
                 rdfs:comment "method used for this save"@en ;
                 rdfs:isDefinedBy sport: ;
                 rdfs:label "save method"@en .


###  https://sportschema.org/ontologies/main/saveType
sport:saveType rdf:type owl:DatatypeProperty ;
               rdfs:domain sport:Action ;
               rdfs:range xsd:string ;
               rdfs:comment "type of save performed in this action"@en ;
               rdfs:isDefinedBy sport: ;
               rdfs:label "save type"@en .


###  https://sportschema.org/ontologies/main/score
sport:score rdf:type owl:DatatypeProperty ;
            rdfs:domain sport:CompetitorParticipation ;
            rdfs:range xsd:string ;
            rdfs:comment "Final or current score of the team or individual"@en ;
            rdfs:isDefinedBy sport: ;
            rdfs:label "score"@en .


###  https://sportschema.org/ontologies/main/scoreAttemptResult
sport:scoreAttemptResult rdf:type owl:DatatypeProperty ;
                         rdfs:domain sport:Action ;
                         rdfs:range <http://www.w3.org/2004/02/skos/core#Concept> ;
                         rdfs:comment "The result of the score attempt eg. blocked, missed, etc. See 'scoreattemptresult' SportsML vocabs for various sports: http://cv.iptc.org/newscodes/spbkbscoreattemptresult/ http://cv.iptc.org/newscodes/spichscoreattemtresult/ http://cv.iptc.org/newscodes/sprgxscoreattemptresult/ http://cv.iptc.org/newscodes/spsocscoreattemptresult/"@en ;
                         rdfs:isDefinedBy sport: ;
                         rdfs:label "score attempt result"@en .


###  https://sportschema.org/ontologies/main/scoreAttemptSide
sport:scoreAttemptSide rdf:type owl:DatatypeProperty ;
                       rdfs:domain sport:Action ;
                       rdfs:range xsd:string ;
                       rdfs:comment "Side of the body of the player attempting to score"@en ;
                       rdfs:isDefinedBy sport: ;
                       rdfs:label "score attempt side"@en .


###  https://sportschema.org/ontologies/main/scoreAttemptSituation
sport:scoreAttemptSituation rdf:type owl:DatatypeProperty ;
                            rdfs:domain sport:Action ;
                            rdfs:range xsd:string ;
                            rdfs:comment "Describing the situation surrounding the score attempt"@en ;
                            rdfs:isDefinedBy sport: ;
                            rdfs:label "score attempt situation"@en .


###  https://sportschema.org/ontologies/main/scoreAttemptType
sport:scoreAttemptType rdf:type owl:DatatypeProperty ;
                       rdfs:domain sport:Action ;
                       rdfs:range <http://www.w3.org/2004/02/skos/core#Concept> ;
                       rdfs:comment "The type of score that was attempted. See 'scoreattempt' SportsML vocabs for various sports: http://cv.iptc.org/newscodes/spbkbscoreattempt/ http://cv.iptc.org/newscodes/spichscoreattempt/ http://cv.iptc.org/newscodes/sprgxscoreattempt/ http://cv.iptc.org/newscodes/spsocscoreattempt/"@en ;
                       rdfs:isDefinedBy sport: ;
                       rdfs:label "score attempt type"@en .


###  https://sportschema.org/ontologies/main/scoreType
sport:scoreType rdf:type owl:DatatypeProperty ;
                rdfs:domain sport:CompetitorParticipation ;
                rdfs:range xsd:string ;
                rdfs:comment "Qualifies the 'score' property."@en ;
                rdfs:isDefinedBy sport: ;
                rdfs:label "score type"@en .


###  https://sportschema.org/ontologies/main/scoreUnits
sport:scoreUnits rdf:type owl:DatatypeProperty ;
                 rdfs:domain sport:CompetitorParticipation ;
                 rdfs:range <http://www.w3.org/2004/02/skos/core#Concept> ;
                 rdfs:comment "The units of a team's or individual's score in a given event (e.g. metres or seconds)"@en ;
                 rdfs:isDefinedBy sport: ;
                 rdfs:label "score units"@en .


###  https://sportschema.org/ontologies/main/sequenceNumber
sport:sequenceNumber rdf:type owl:DatatypeProperty ;
                     rdfs:domain sport:Action ;
                     rdfs:range xsd:string ;
                     rdfs:comment "Sequence-number. Should be separate sequences for sub-actions inside an action"@en ;
                     rdfs:isDefinedBy sport: ;
                     rdfs:label "sequence number"@en .


###  https://sportschema.org/ontologies/main/shotDistance
sport:shotDistance rdf:type owl:DatatypeProperty ;
                   rdfs:domain sport:Action ;
                   rdfs:range xsd:string ;
                   rdfs:comment "Distance of the shot"@en ;
                   rdfs:isDefinedBy sport: ;
                   rdfs:label "shot distance"@en .


###  https://sportschema.org/ontologies/main/shotDistanceUnits
sport:shotDistanceUnits rdf:type owl:DatatypeProperty ;
                        rdfs:domain sport:Action ;
                        rdfs:range <http://www.w3.org/2004/02/skos/core#Concept> ;
                        rdfs:comment "SportsML vocab uri: http://cv.iptc.org/newscodes/spdistanceunits/"@en ;
                        rdfs:isDefinedBy sport: ;
                        rdfs:label "shot distance units"@en .


###  https://sportschema.org/ontologies/main/shotType
sport:shotType rdf:type owl:DatatypeProperty ;
               rdfs:domain sport:Action ;
               rdfs:range <http://www.w3.org/2004/02/skos/core#Concept> ;
               rdfs:comment "The type of shot taken. See 'shot' SportsML vocabs for various sports: http://cv.iptc.org/newscodes/spgolshot/ http://cv.iptc.org/newscodes/sptenshot/ http://cv.iptc.org/newscodes/spcurshot/"@en ;
               rdfs:isDefinedBy sport: ;
               rdfs:label "shot type"@en .


###  https://sportschema.org/ontologies/main/sport
sport:sport rdf:type owl:DatatypeProperty ;
            rdfs:domain sport:Competition ;
            rdfs:range xsd:anyURI ,
                       <http://www.w3.org/2004/02/skos/core#Concept> ;
            rdfs:comment "The sport which this competition represents"@en ;
            rdfs:isDefinedBy sport: ;
            rdfs:label "sport"@en .


###  https://sportschema.org/ontologies/main/startDate
sport:startDate rdf:type owl:DatatypeProperty ;
                rdfs:domain sport:Membership ;
                rdfs:range xsd:date ;
                rdfs:comment "The date on which a membership begins"@en ;
                rdfs:isDefinedBy sport: ;
                rdfs:label "start date"@en .


###  https://sportschema.org/ontologies/main/startDateTime
sport:startDateTime rdf:type owl:DatatypeProperty ;
                    rdfs:domain sport:Event ;
                    rdfs:range xsd:dateTime ;
                    rdfs:comment "The date and time at which an event begins"@en ;
                    rdfs:isDefinedBy sport: ;
                    rdfs:label "start datetime"@en .


###  https://sportschema.org/ontologies/main/startLocation
sport:startLocation rdf:type owl:DatatypeProperty ;
                    rdfs:domain sport:Action ;
                    rdfs:range xsd:string ;
                    rdfs:comment ">A string indicating where on the court the action began. Could be an approximate region, or a more complex value adhering to some elaborate coordinate system."@en ;
                    rdfs:isDefinedBy sport: ;
                    rdfs:label "start location"@en .


###  https://sportschema.org/ontologies/main/substitutionReason
sport:substitutionReason rdf:type owl:DatatypeProperty ;
                         rdfs:domain sport:Action ;
                         rdfs:range xsd:string ;
                         rdfs:comment "The reason for the substitution of a player"@en ;
                         rdfs:isDefinedBy sport: ;
                         rdfs:label "substitution reason"@en .


###  https://sportschema.org/ontologies/main/timeAddition
sport:timeAddition rdf:type owl:DatatypeProperty ;
                   rdfs:domain sport:Action ;
                   rdfs:range xsd:string ;
                   rdfs:comment "time added to period."@en ;
                   rdfs:isDefinedBy sport: ;
                   rdfs:label "time addition"@en .


###  https://sportschema.org/ontologies/main/timeElapsed
sport:timeElapsed rdf:type owl:DatatypeProperty ;
                  rdfs:domain sport:Action ;
                  rdfs:range xsd:string ;
                  rdfs:comment "Total time elapsed of event"@en ;
                  rdfs:isDefinedBy sport: ;
                  rdfs:label "time elapsed"@en .


###  https://sportschema.org/ontologies/main/timeRemaining
sport:timeRemaining rdf:type owl:DatatypeProperty ;
                    rdfs:domain sport:Action ;
                    rdfs:range xsd:string ;
                    rdfs:comment "Time remaining of event"@en ;
                    rdfs:isDefinedBy sport: ;
                    rdfs:label "time remaining"@en .


###  https://sportschema.org/ontologies/main/uniformNumber
sport:uniformNumber rdf:type owl:DatatypeProperty ;
                    rdfs:domain sport:IndividualMembership ;
                    rdfs:range xsd:string ;
                    rdfs:comment "The number usually worn on a player's uniform (jersey etc.) Note that the value may be a string such as 'unknown'."@en ;
                    rdfs:isDefinedBy sport: ;
                    rdfs:label "uniform number"@en .


###  https://sportschema.org/ontologies/main/uniformNumberEvent
sport:uniformNumberEvent rdf:type owl:DatatypeProperty ;
                         rdfs:domain sport:IndividualParticipation ;
                         rdfs:range xsd:string ;
                         rdfs:comment "The number worn on a player's uniform (jersey etc.) for an individual event. Note that the value may be a string such as 'unknown'."@en ;
                         rdfs:isDefinedBy sport: ;
                         rdfs:label "uniform number event"@en .


###  https://sportschema.org/ontologies/main/zone
sport:zone rdf:type owl:DatatypeProperty ;
           rdfs:domain sport:Action ;
           rdfs:range xsd:string ;
           rdfs:comment "The zone on the playing field where the action took place. Value can be sport specific"@en ;
           rdfs:isDefinedBy sport: ;
           rdfs:label "zone"@en .


#################################################################
#    Classes
#################################################################

###  https://sportschema.org/ontologies/main/Action
sport:Action rdf:type owl:Class ;
             rdfs:subClassOf sport:ParticipatableThing ;
             rdfs:comment "Something that happens during an event: a kick, a goal, a foul etc"@en ;
             rdfs:isDefinedBy sport: ;
             rdfs:label "Action"@en .


###  https://sportschema.org/ontologies/main/Agent
sport:Agent rdf:type owl:Class ;
            rdfs:comment "A participant in a sport event."@en ;
            rdfs:isDefinedBy sport: ;
            rdfs:label "Agent"@en .


###  https://sportschema.org/ontologies/main/Associate
sport:Associate rdf:type owl:Class ;
                rdfs:subClassOf sport:Individual ;
                rdfs:comment "A person assisting competitor(s) in an event but not competing themselves, e.g. a football manager or coach"@en ;
                rdfs:isDefinedBy sport: ;
                rdfs:label "Associate"@en .


###  https://sportschema.org/ontologies/main/AssociateParticipation
sport:AssociateParticipation rdf:type owl:Class ;
                             rdfs:subClassOf sport:Participation ;
                             rdfs:comment "The particpation of an associate who supports players and teams, e.g. coach, manager, trainer"@en ;
                             rdfs:isDefinedBy sport: ;
                             rdfs:label "Associate Participation"@en .


###  https://sportschema.org/ontologies/main/Athlete
sport:Athlete rdf:type owl:Class ;
              rdfs:subClassOf sport:Individual ;
              rdfs:comment "A competitor in an individual event or a member of a team"@en ;
              rdfs:isDefinedBy sport: ;
              rdfs:label "Athlete"@en .


###  https://sportschema.org/ontologies/main/Competition
sport:Competition rdf:type owl:Class ;
                  rdfs:subClassOf sport:ParticipatableThing ;
                  rdfs:comment "A grouping of events usually based on proximity by time."@en ;
                  rdfs:isDefinedBy sport: ;
                  rdfs:label "Competition"@en .


###  https://sportschema.org/ontologies/main/CompetitionPhase
sport:CompetitionPhase rdf:type owl:Class ;
                       rdfs:subClassOf sport:Competition ;
                       rdfs:comment "A sub-group of events within a Competition such as the semi-finals."@en ;
                       rdfs:isDefinedBy sport: ;
                       rdfs:label "Competition Phase"@en .


###  https://sportschema.org/ontologies/main/CompetitorParticipation
sport:CompetitorParticipation rdf:type owl:Class ;
                              rdfs:subClassOf sport:Participation ;
                              rdfs:comment "The participation of an actor that can win or lose an event."@en ;
                              rdfs:isDefinedBy sport: ;
                              rdfs:label "Competitor Participation"@en .


###  https://sportschema.org/ontologies/main/Event
sport:Event rdf:type owl:Class ;
            rdfs:subClassOf sport:ParticipatableThing ;
            rdfs:comment "A contest of competitive actions that generates statistical results."@en ;
            rdfs:isDefinedBy sport: ;
            rdfs:label "Event"@en .


###  https://sportschema.org/ontologies/main/GoverningBody
sport:GoverningBody rdf:type owl:Class ;
                    rdfs:comment "The organisation that creates and polices the rules of a sports competition."@en ;
                    rdfs:isDefinedBy sport: ;
                    rdfs:label "Governing Body"@en .


###  https://sportschema.org/ontologies/main/Individual
sport:Individual rdf:type owl:Class ;
                 rdfs:subClassOf sport:Agent ;
                 rdfs:comment "An individual taking part in an event on their own or as part of a team. Could be a person or an animal such as a dog or horse."@en ;
                 rdfs:isDefinedBy sport: ;
                 rdfs:label "Individual"@en .


###  https://sportschema.org/ontologies/main/IndividualMembership
sport:IndividualMembership rdf:type owl:Class ;
                           rdfs:subClassOf sport:Membership ;
                           rdfs:comment "A player's membership in a team"@en ;
                           rdfs:isDefinedBy sport: ;
                           rdfs:label "Individual Membership"@en .


###  https://sportschema.org/ontologies/main/IndividualParticipation
sport:IndividualParticipation rdf:type owl:Class ;
                              rdfs:subClassOf sport:CompetitorParticipation ;
                              rdfs:comment "The participation of an individual in an event"@en ;
                              rdfs:isDefinedBy sport: ;
                              rdfs:label "Individual Participation"@en .


###  https://sportschema.org/ontologies/main/Membership
sport:Membership rdf:type owl:Class ;
                 rdfs:comment "The membership of an entity in another entity for a given period of time"@en ;
                 rdfs:isDefinedBy sport: ;
                 rdfs:label "Membership"@en .


###  https://sportschema.org/ontologies/main/Official
sport:Official rdf:type owl:Class ;
               rdfs:subClassOf sport:Individual ;
               rdfs:comment "A person who ensures that the sports event is played according to its rules. Also referred to as umpire or referee."@en ;
               rdfs:isDefinedBy sport: ;
               rdfs:label "Official"@en .


###  https://sportschema.org/ontologies/main/OfficialParticipation
sport:OfficialParticipation rdf:type owl:Class ;
                            rdfs:subClassOf sport:Participation ;
                            rdfs:comment "The participation of an offcial in an event"@en ;
                            rdfs:isDefinedBy sport: ;
                            rdfs:label "Official Participation"@en .


###  https://sportschema.org/ontologies/main/ParticipatableThing
sport:ParticipatableThing rdf:type owl:Class ;
                          rdfs:comment "An abstract superclass for anything that can be participated in, such as an Event, Competition or Action."@en ;
                          rdfs:isDefinedBy sport: ;
                          rdfs:label "Participatable Thing"@en .


###  https://sportschema.org/ontologies/main/Participation
sport:Participation rdf:type owl:Class ;
                    rdfs:comment "The participation of an actor in an event."@en ;
                    rdfs:isDefinedBy sport: ;
                    rdfs:label "Participation"@en .


###  https://sportschema.org/ontologies/main/ParticipationSplit
sport:ParticipationSplit rdf:type owl:Class ;
                         rdfs:comment "Representation of part of a participation of an actor in an event or season, such as one half of a football match or all home games."@en ;
                         rdfs:isDefinedBy sport: ;
                         rdfs:label "Participation Split"@en .


###  https://sportschema.org/ontologies/main/Site
sport:Site rdf:type owl:Class ;
           rdfs:comment "The location where an activity takes place"@en ;
           rdfs:isDefinedBy sport: ;
           rdfs:label "Site"@en .


###  https://sportschema.org/ontologies/main/Team
sport:Team rdf:type owl:Class ;
           rdfs:subClassOf sport:Agent ;
           rdfs:comment "A group of individuals competing as one entity"@en ;
           rdfs:isDefinedBy sport: ;
           rdfs:label "Team"@en .


###  https://sportschema.org/ontologies/main/TeamParticipation
sport:TeamParticipation rdf:type owl:Class ;
                        rdfs:subClassOf sport:CompetitorParticipation ;
                        rdfs:comment "The participation of a team in an event"@en ;
                        rdfs:isDefinedBy sport: ;
                        rdfs:label "Team Participation"@en .


###  https://sportschema.org/ontologies/main/event
sport:event rdf:type owl:Class .


#################################################################
#    Annotations
#################################################################

spstat:resultEffectTarget rdfs:comment "The Competition/Event that the resultEffect gains access to, e.g. for qualification for a final the target would be the Event of the final, for relegation in soccer the target would be the new league division."@en ;
                          rdfs:label "resultEffectTarget"@en .


###  Generated by the OWL API (version 4.5.26.2023-07-17T20:34:13Z) https://github.com/owlcs/owlapi
